failing attempt to do Cenv_bs_change_store_and_refs
Was assuming, while doing this, that RefPtrs in an environment must be
pointers to recursive closures (and hence can't change), but that's not
true: there can be ordinary refs there too. So need to go back and prove
a more careful version of lookup_ct_change_refs...

compiler/correctness/compileCorrectnessScript.sml
@@ -326,7 +326,8 @@ val good_cls_def = Define`
 val s_refs_def = Define`
   s_refs c sm cls s bs =
   fmap_rel (Cv_bv (mk_pp (DRESTRICT sm (FDOM s)) c bs cls)) s
-  (DRESTRICT bs.refs (FRANGE (DRESTRICT sm (FDOM s))))`
+  (DRESTRICT bs.refs (FRANGE (DRESTRICT sm (FDOM s)))) ∧
+  ∀vs p. MEM (Block 0 vs) bs.stack ∧ MEM (RefPtr p) vs ⇒ p ∈ FDOM bs.refs ∧ p ∉ FRANGE (DRESTRICT sm (FDOM s))`
 
 val Cenv_bs_def = Define`
   Cenv_bs c sm cls s Cenv (renv:ctenv) sz bs =
@@ -969,14 +970,18 @@ val lookup_ct_imp_incsz = store_thm("lookup_ct_imp_incsz",
 
 val Cenv_bs_imp_incsz = store_thm("Cenv_bs_imp_incsz",
   ``∀c sm cls s env renv rsz bs bs'.
-    Cenv_bs c sm cls s env renv rsz bs ∧ (∃v p e. bs' = bs with <| stack := v::bs.stack; pc := p; exstack := e |>) ⇒
+    Cenv_bs c sm cls s env renv rsz bs ∧
+    (∃v p e. (bs' = bs with <| stack := v::bs.stack; pc := p; exstack := e |>) ∧
+             ∀vs p. (v = Block 0 vs) ∧ (MEM (RefPtr p) vs) ⇒ p ∈ FDOM bs.refs ∧ p ∉ FRANGE (DRESTRICT sm (FDOM s)))
+    ⇒
     Cenv_bs c sm cls s env renv (rsz+1) bs'``,
-  rw[Cenv_bs_def,fmap_rel_def,s_refs_def,FDOM_DRESTRICT] >> rw[] >>
-  qmatch_assum_rename_tac `z ∈ FDOM env`[] >>
-  first_x_assum (qspec_then `z` mp_tac) >>
-  BasicProvers.CASE_TAC >>
-  imp_res_tac lookup_ct_imp_incsz >>
-  rw[] )
+  rw[Cenv_bs_def,fmap_rel_def,s_refs_def,FDOM_DRESTRICT] >> rw[] >> fs[] >- (
+    qmatch_assum_rename_tac `z ∈ FDOM env`[] >>
+    first_x_assum (qspec_then `z` mp_tac) >>
+    BasicProvers.CASE_TAC >>
+    imp_res_tac lookup_ct_imp_incsz >>
+    rw[] ) >>
+  metis_tac[])
 
 val Cenv_bs_imp_decsz = store_thm("Cenv_bs_imp_decsz",
   ``∀c sm cls s env renv rsz bs bs'.
@@ -984,14 +989,15 @@ val Cenv_bs_imp_decsz = store_thm("Cenv_bs_imp_decsz",
       (CTLet (rsz+1) ∉ FRANGE renv) ∧
       (∃v p e. bs = bs' with <| stack := v::bs'.stack; pc := p; exstack := e |>) ⇒
     Cenv_bs c sm cls s env renv rsz bs'``,
-  rw[Cenv_bs_def,fmap_rel_def,s_refs_def,FDOM_DRESTRICT] >> fs[] >>
-  qmatch_assum_rename_tac `z ∈ FDOM env`[] >>
-  first_x_assum (qspec_then `z` mp_tac) >>
-  BasicProvers.CASE_TAC >>
-  pop_assum mp_tac >>
-  rw[lookup_ct_incsz] >>
-  fs[FRANGE_DEF] >>
-  PROVE_TAC[])
+  rw[Cenv_bs_def,fmap_rel_def,s_refs_def,FDOM_DRESTRICT] >> fs[] >- (
+    qmatch_assum_rename_tac `z ∈ FDOM env`[] >>
+    first_x_assum (qspec_then `z` mp_tac) >>
+    BasicProvers.CASE_TAC >>
+    pop_assum mp_tac >>
+    rw[lookup_ct_incsz] >>
+    fs[FRANGE_DEF] >>
+    PROVE_TAC[]) >>
+  metis_tac[])
 
 val Cenv_bs_CTLet_bound = store_thm("Cenv_bs_CTLet_bound",
   ``Cenv_bs c sm cls s env renv rsz bs ∧ CTLet n ∈ FRANGE renv ⇒ n ≤ rsz``,
@@ -1006,7 +1012,7 @@ val Cenv_bs_pops = store_thm("Cenv_bs_pops",
     (∀n. CTLet n ∈ FRANGE renv ⇒ n ≤ rsz) ∧
     (∃p e. bs = bs' with <| stack := vs ++ bs'.stack; pc := p; exstack := e|>)
     ⇒ Cenv_bs c sm cls s env renv rsz bs'``,
-  Induct >> rw[] >- ( fs[Cenv_bs_def,s_refs_def] ) >>
+  Induct >> rw[] >- ( fs[Cenv_bs_def,s_refs_def] >> fs[]) >>
   first_x_assum match_mp_tac >>
   simp[bc_state_component_equality] >>
   qexists_tac`bs' with stack := vs ++ bs'.stack` >> rw[] >>
@@ -1020,10 +1026,6 @@ val Cenv_bs_pops = store_thm("Cenv_bs_pops",
 
 val s_refs_with_pc = store_thm("s_refs_with_pc",
   ``s_refs c sm cls s (bs with pc := p) = s_refs c sm cls s bs``,
-  rw[s_refs_def])
-
-val s_refs_with_stack = store_thm("s_refs_with_stack",
-  ``s_refs c sm cls s (bs with stack := p) = s_refs c sm cls s bs``,
   rw[s_refs_def])
 
 val Cenv_bs_with_pc = store_thm("Cenv_bs_with_pc",
@@ -1510,19 +1512,21 @@ val Cenv_bs_FUPDATE = store_thm("Cenv_bs_FUPDATE",
   ``∀c sm cls s env env0 sz0 bs n v bv bs'.
     Cenv_bs c sm cls s env env0 sz0 bs ∧
     Cv_bv (mk_pp (DRESTRICT sm (FDOM s)) c bs' cls) v bv ∧
-    (bs' = bs with stack := bv::bs.stack)
+    (bs' = bs with stack := bv::bs.stack) ∧
+    (∀vs p. (bv = Block 0 vs) ∧ (MEM (RefPtr p) vs) ⇒ p ∈ FDOM bs.refs ∧ p ∉ FRANGE (DRESTRICT sm (FDOM s)))
     ⇒
     Cenv_bs c sm cls s (env |+ (n,v)) (env0 |+ (n,CTLet (sz0 + 1))) (sz0 + 1) bs'``,
-  rw[Cenv_bs_def,s_refs_def] >>
-  fs[fmap_rel_def] >>
-  qx_gen_tac`x` >>
-  Cases_on`x=n`>>fs[] >>
-  strip_tac >>
-  rw[FAPPLY_FUPDATE_THM] >>
-  first_x_assum (qspec_then `x` mp_tac) >> rw[] >>
-  Cases_on `lookup_ct sz0 bs.stack bs.refs (env0 ' x)` >> fs[] >>
-  imp_res_tac lookup_ct_imp_incsz >>
-  pop_assum (qspec_then`bv`mp_tac) >> rw[])
+  rw[Cenv_bs_def,s_refs_def] >> fs[] >- (
+    fs[fmap_rel_def] >>
+    qx_gen_tac`x` >>
+    Cases_on`x=n`>>fs[] >>
+    strip_tac >>
+    rw[FAPPLY_FUPDATE_THM] >>
+    first_x_assum (qspec_then `x` mp_tac) >> rw[] >>
+    Cases_on `lookup_ct sz0 bs.stack bs.refs (env0 ' x)` >> fs[] >>
+    imp_res_tac lookup_ct_imp_incsz >>
+    pop_assum (qspec_then`bv`mp_tac) >> rw[]) >>
+  metis_tac[])
 
 val Cenv_bs_DOMSUB = store_thm("Cenv_bs_DOMSUB",
   ``∀c sm cls s env k renv rsz bs.
@@ -1673,33 +1677,39 @@ val Cv_bv_SUBMAP = store_thm("Cv_bv_SUBMAP",
   Q.PAT_ABBREV_TAC`evs = FILTER X (SET_TO_LIST fvs)` >>
   fs[] >> metis_tac[])
 
+val lookup_ct_change_refs = store_thm("lookup_ct_change_refs",
+  ``∀sz st rf rf'.
+    let s = { p | ∃vs. MEM (Block 0 vs) st ∧ MEM (RefPtr p) vs } in
+    (DRESTRICT rf s = DRESTRICT rf' s)
+    ⇒ (lookup_ct sz st rf' = lookup_ct sz st rf)``,
+  rw[FUN_EQ_THM,LET_THM] >>
+  Cases_on`x`>>fs[] >> rw[] >>
+  Cases_on`EL sz st`>>fs[] >>
+  rw[]>>fs[]>>
+  BasicProvers.CASE_TAC>>fs[]>>
+  BasicProvers.CASE_TAC>>fs[]>>
+  fs[GSYM fmap_EQ_THM,DRESTRICT_DEF,FLOOKUP_DEF,MEM_EL,EXTENSION] >>
+  rw[] >> metis_tac[])
+
 val Cenv_bs_change_store = store_thm("Cenv_bs_change_store",
-  ``∀c sm cls s env renv rsz bs s'.
+  ``∀c sm cls s env renv rsz bs s' bs' rfs'.
     Cenv_bs c sm cls s env renv rsz bs ∧
-    s_refs c sm cls s' bs ∧
+    s_refs c sm cls s' bs' ∧
+    (bs' = bs with refs := rfs') ∧
+    (let ps = { p | ∃vs. MEM (Block 0 vs) bs.stack ∧ MEM (RefPtr p) vs } in (DRESTRICT bs.refs ps = DRESTRICT rfs' ps)) ∧
     FDOM s ⊆ FDOM s' ∧
     (∀p. p ∈ FDOM cls ∧ p ∉ FRANGE (DRESTRICT sm (FDOM s)) ⇒ p ∉ FRANGE (DRESTRICT sm (FDOM s')))
     ⇒
-    Cenv_bs c sm cls s' env renv rsz bs``,
+    Cenv_bs c sm cls s' env renv rsz bs'``,
   rw[Cenv_bs_def,fmap_rel_def] >>
   first_x_assum(qspec_then`x`mp_tac) >> rw[] >>
+  qspecl_then[`rsz`,`bs.stack`,`bs.refs`,`rfs'`]mp_tac lookup_ct_change_refs >>
+  fs[LET_THM] >> rw[] >>
   BasicProvers.EVERY_CASE_TAC >> fs[] >>
   match_mp_tac (MP_CANON (GEN_ALL (CONJUNCT1 (SPEC_ALL Cv_bv_SUBMAP)))) >>
   simp[] >>
   qexists_tac`DRESTRICT sm (FDOM s)` >>
   fs[SUBMAP_DEF,SUBSET_DEF,DRESTRICT_DEF])
-
-val Cenv_bs_change_refs = store_thm("Cenv_bs_change_refs",
-  ``∀c sm cls s env renv rsz bs bs' rfs'.
-    Cenv_bs c sm cls s env renv rsz bs ∧
-    (bs' = bs with refs := rfs') ∧
-    s_refs c sm cls s bs' ∧
-    all block 0s inside (EL sz st) have refptrs outside the range of sm ∧
-    rfs' extends rfs on things outside the range of sm
-    ⇒
-    Cenv_bs c sm cls s env renv rsz bs'``,
-  rw[Cenv_bs_def,fmap_rel_def] >>
-  lookup_ct_def
 
 val good_sm_DRESTRICT = store_thm("good_sm_DRESTRICT",
   ``good_sm sm ⇒ good_sm (DRESTRICT sm s)``,
@@ -1900,6 +1910,7 @@ val code_for_push_return = store_thm("code_for_push_return",
     qmatch_assum_rename_tac `Cv_bv pp v bv`["pp"] >>
     map_every qexists_tac [`bv`,`rf`] >>
     fs[Cenv_bs_def,s_refs_def,good_cls_def] >>
+    reverse conj_tac >- METIS_TAC[] >>
     qmatch_assum_abbrev_tac`bc_next^* bs0 bs1` >>
     qspecl_then[`bs0`,`bs1`,`retbc 1 (LENGTH args) ++ bc1`]mp_tac (SIMP_RULE(srw_ss())[]RTC_bc_next_append_code) >>
     rw[] >>
@@ -2550,7 +2561,23 @@ val benv_bvs_free_vars_SUBSET = store_thm("benv_bvs_free_vars_SUBSET",
   pop_assum(strip_assume_tac o SIMP_RULE(srw_ss())[MEM_EL]) >>
   first_x_assum(qspec_then`n`mp_tac) >> rw[])
 
+val benv_bvs_good_env = store_thm("benv_bvs_good_benv",
+  ``benv_bvs pp benv fvs xs env defs ns i ⇒
+    ∀vs p. (benv = Block 0 vs) ∧ MEM (RefPtr p) vs ⇒
+    p ∈ FDOM (SND(SND(SND pp)))``,
+  simp[Once Cv_bv_cases] >>
+  rw[] >> fs[] >>
+  BasicProvers.EVERY_CASE_TAC >> fs[] >> rw[] >>
+  fs[MEM_EL] >>
+  first_x_assum(qspec_then`n`mp_tac)>>rw[]>>rfs[]>>fs[FLOOKUP_DEF]>>
+  qpat_assum`X = EL n bvs`(assume_tac o SYM) >>fs[Once Cv_bv_cases]
+  Cv_bv_rules
+
 fun filter_asms P = POP_ASSUM_LIST (MAP_EVERY ASSUME_TAC o List.rev o List.filter P)
+
+val Cv_bv_not_env = store_thm("Cv_bv_not_env",
+  ``∀pp Cv bv. Cv_bv pp Cv bv ⇒ ∀vs. (bv = Block 0 vs) ⇒ (vs = [])``,
+  gen_tac >> ho_match_mp_tac Cv_bv_only_ind >> simp[])
 
 val compile_val = store_thm("compile_val",
   ``(∀c d s env exp res. Cevaluate c d s env exp res ⇒
@@ -2618,7 +2645,8 @@ val compile_val = store_thm("compile_val",
       REWRITE_TAC[Once option_case_NONE_F] >> simp[] >>
       disch_then(Q.X_CHOOSE_THEN`x`strip_assume_tac) >>
       strip_tac >>
-      map_every qexists_tac [`[x]`,`bs.refs`] >> rw[s_refs_with_stack] >- (
+      imp_res_tac Cv_bv_not_env >>
+      map_every qexists_tac [`[x]`,`bs.refs`] >> rw[] >- (
         match_mp_tac compile_varref_thm >> fs[] >>
         simp[bc_state_component_equality] >>
         metis_tac[])
@@ -2631,6 +2659,8 @@ val compile_val = store_thm("compile_val",
         qunabbrev_tac`X` >>
         imp_res_tac lookup_ct_imp_incsz >>
         rw[] )
+      >- (
+        fs[s_refs_def] >> rw[] >> fs[] >> PROVE_TAC[])
       >- (
         REWRITE_TAC[GSYM BytecodeTheory.bc_state_fupdcanon] >>
         rw[s_refs_with_pc]) >>
@@ -2835,7 +2865,10 @@ val compile_val = store_thm("compile_val",
       qunabbrev_tac`sz1` >>
       match_mp_tac Cenv_bs_imp_incsz >>
       qexists_tac`bs1 with stack := bs.stack` >>
-      rw[bc_state_component_equality,Abbr`bs1`] ) >>
+      simp[bc_state_component_equality,Abbr`bs1`] >>
+      first_x_assum(qspec_then`n`mp_tac) >> simp[] >>
+      strip_tac >> imp_res_tac Cv_bv_not_env >>
+      rw[] >> fs[] >> rw[] >> fs[]) >>
     first_x_assum(qspec_then`sm` kall_tac) >>
     fs[compile_def,LET_THM] >>
     rw[]>>fs[] >>
@@ -3231,7 +3264,15 @@ val compile_val = store_thm("compile_val",
           map_every qexists_tac[`a`,`bvs`,`bs.stack`] >>
           simp[] >>
           conj_tac >- fs[good_cls_def] >>
-          conj_tac >- fs[s_refs_def,Cenv_bs_def] >>
+          conj_tac >- (
+            fs[s_refs_def,Cenv_bs_def] >>
+            map_every qx_gen_tac[`ws`,`p`] >>
+            strip_tac >- (
+              qpat_assum`benv_bvs X bve Y xs env' defs ns' i`mp_tac >>
+
+              simp[Once Cv_bv_cases]
+            rpt gen_tac
+
           conj_tac >- (rw[] >> fs[]) >>
           conj_tac >- (rw[] >> fs[]) >>
           fs[FLOOKUP_DEF] >> rfs[] >>
@@ -3266,18 +3307,27 @@ val compile_val = store_thm("compile_val",
       simp[Abbr`P`] >>
       reverse conj_tac >- PROVE_TAC[SUBMAP_TRANS] >>
       match_mp_tac Cenv_bs_imp_incsz >>
+      qunabbrev_tac`bs0` >>
       qmatch_assum_abbrev_tac`Cenv_bs c sm cls s cenv cs.env cs.sz bs0` >>
       qexists_tac`bs0 with refs := rfr` >>
       simp[Abbr`bs0`,bc_state_component_equality] >>
+      match_mp_tac Cenv_bs_change_store >>
+      qmatch_assum_abbrev_tac`Cenv_bs c sm cls s cenv cs.env cs.sz bs0` >>
+      map_every qexists_tac[`s`,`bs0`] >>
+      simp[] >>
+      fs[s_refs_def,Abbr`l2a`] >>
+      simp[Abbr`bs0`,bc_state_component_equality] >>
+      `FDOM s ⊆ FDOM s'''` by metis_tac[SUBSET_TRANS] >>
+
+      simp[]
+      DRESTRICT_EQ_DRESTRICT_SAME
+      DB.find"DRESTRICT_EQ_"
 
       Cenv_bs_def
       Cenv_bs_change_store
       simp[Cenv_bs_def] >>
 
-
-
-
-      filter_asms (can (find_term (equal ``Cenv_bs``)) o concl)
+      filter_asms (can (find_term (equal (SOME "cls") o Option.map fst o total dest_var)) o concl)
       set_trace "goalstack print goal at top" 0
 
     (* >>
